Inductions for tangle attractors
These do not quite do what I want them to, but they might be a step in the right direction.

TangleAttractors.thy
@@ -1,87 +1,77 @@
 theory TangleAttractors
-imports Main Tangles
+  imports Main Tangles
 begin
 chapter \<open>Tangle Attractors\<close>
 section \<open>Tangle Attractors for Arbitrary Players\<close>
 context player_paritygame begin
-(** We fix the set of known tangles T. *)
+  (** We fix the set of known tangles T. *)
 context
   fixes T :: "'v set set"
   assumes tangles_T: "\<forall>t\<in>T. player_tangle t"
   assumes fin_T: "finite T"
 begin
-subsection \<open>Tangle Attractors as Inductive Sets\<close>
-inductive_set player_tangle_attractor :: "'v set \<Rightarrow> 'v set" for A where
-  base: "x \<in> A \<Longrightarrow> x \<in> player_tangle_attractor A"
-| own: "\<lbrakk>x \<in> V\<^sub>\<alpha>-A; (x,y) \<in> E; y \<in> player_tangle_attractor A\<rbrakk> \<Longrightarrow> x \<in> player_tangle_attractor A"
-| opponent: "\<lbrakk>x \<in> V\<^sub>\<beta>-A; \<forall>y. (x,y) \<in> E \<longrightarrow> y \<in> player_tangle_attractor A\<rbrakk>
-              \<Longrightarrow> x \<in> player_tangle_attractor A"
-| escape: "\<lbrakk>x \<in> t; t \<in> T; t \<inter> A = {}; opponent_escapes t \<noteq> {};
-            \<forall>v. v \<in> opponent_escapes t \<longrightarrow> v \<in> player_tangle_attractor A\<rbrakk>
-            \<Longrightarrow> x \<in> player_tangle_attractor A"
-
-lemma A_in_player_tangle_attractor: "A \<subseteq> player_tangle_attractor A"
-  using player_tangle_attractor.base by fast
-
-lemma player_tangle_attractor_ss: "player_tangle_attractor A \<subseteq> A \<union> V"
-  using tangles_T in_mono V\<^sub>\<alpha>_subset DiffE
-  unfolding player_tangle_def
-  apply (auto intro: player_tangle_attractor.cases)
-  by (smt (verit) DiffE V\<^sub>\<alpha>_subset in_mono player_tangle_attractor.cases)
-  (** This needs improvement *)
-
-definition player_tangle_attractor_strat :: "'v strat \<Rightarrow> 'v set \<Rightarrow> bool" where
-  "player_tangle_attractor_strat \<sigma> A \<equiv>
-    strategy_of V\<^sub>\<alpha> \<sigma> \<and>
-    dom \<sigma> = V\<^sub>\<alpha> \<inter> (player_tangle_attractor A - A) \<and>
-    ran \<sigma> \<subseteq> player_tangle_attractor A \<and>
-    induced_subgraph V\<^sub>\<alpha> \<sigma> `` (player_tangle_attractor A - A) \<subseteq> player_tangle_attractor A \<and>
-    (\<forall>x\<in>player_tangle_attractor A. \<forall>xs ys. lasso_from_node (induced_subgraph V\<^sub>\<alpha> \<sigma>) x xs ys
-        \<longrightarrow> (set (xs@ys) \<inter> A \<noteq> {} \<or> winning_player ys))"
 
 subsection \<open>Tangle Attractors as an Inductive Predicate\<close>
 context
   fixes A :: "'v set"
 begin
-inductive attractor_step :: "'v set \<Rightarrow> 'v set \<Rightarrow> bool" where
-  own: "\<lbrakk>x \<in> V\<^sub>\<alpha>-S; (x,y) \<in> E; y \<in> S\<rbrakk> \<Longrightarrow> attractor_step S (insert x S)"
-| opponent: "\<lbrakk>x \<in> V\<^sub>\<beta>-S; \<forall>y. (x,y) \<in> E \<longrightarrow> y \<in> S\<rbrakk> \<Longrightarrow> attractor_step S (insert x S)"
-| escape: "\<lbrakk>t \<in> T; t-S \<noteq> {}; opponent_escapes t \<noteq> {}; opponent_escapes t \<subseteq> S\<rbrakk>
-              \<Longrightarrow> attractor_step S (S \<union> t)"
 
-(** A version of the attractor step where we include the strategy. *)
-inductive attractor_step_strat :: "'v set \<Rightarrow> 'v strat \<Rightarrow> 'v set \<Rightarrow> 'v strat \<Rightarrow> bool" where
-  own: "\<lbrakk>x \<in> V\<^sub>\<alpha>-S; (x,y) \<in> E; y \<in> S\<rbrakk> \<Longrightarrow> attractor_step_strat S \<sigma> (insert x S) (\<sigma>(x\<mapsto>y))"
-| opponent: "\<lbrakk>x \<in> V\<^sub>\<beta>-S; \<forall>y. (x,y) \<in> E \<longrightarrow> y \<in> S\<rbrakk> \<Longrightarrow> attractor_step_strat S \<sigma> (insert x S) \<sigma>"
+inductive tangle_attractor_step :: "'v set \<times> 'v strat \<Rightarrow> 'v set \<times> 'v strat \<Rightarrow> bool" where
+  own: "\<lbrakk>x \<in> V\<^sub>\<alpha>-S; (x,y) \<in> E; y \<in> S\<rbrakk> \<Longrightarrow> tangle_attractor_step (S,\<sigma>) (insert x S,\<sigma>(x\<mapsto>y))"
+| opponent: "\<lbrakk>x \<in> V\<^sub>\<beta>-S; \<forall>y. (x,y) \<in> E \<longrightarrow> y \<in> S\<rbrakk> \<Longrightarrow> tangle_attractor_step (S,\<sigma>) (insert x S,\<sigma>)"
 | escape: "\<lbrakk>t \<in> T; t-S \<noteq> {}; opponent_escapes t \<noteq> {}; opponent_escapes t \<subseteq> S;
-            player_tangle_strat t \<sigma>'\<rbrakk> \<Longrightarrow> attractor_step_strat S \<sigma> (S \<union> t) ((\<sigma>' |` (t-A)) ++ \<sigma>)"
+            player_tangle_strat t \<sigma>'\<rbrakk> \<Longrightarrow> tangle_attractor_step (S,\<sigma>) (S\<union>t,(\<sigma>' |` (t-A)) ++ \<sigma>)"
 
-definition attractor_step_strat_I :: "'v set \<Rightarrow> 'v strat \<Rightarrow> bool" where
-  "attractor_step_strat_I S \<sigma> \<equiv>
+lemma tangle_attractor_step_mono: "tangle_attractor_step S S' \<Longrightarrow> fst S \<subset> fst S'"
+  by (induction rule: tangle_attractor_step.induct) auto
+
+lemma tangle_attractor_step_rtranclp_mono: "tangle_attractor_step\<^sup>*\<^sup>* S S' \<Longrightarrow> fst S \<subseteq> fst S'"
+  apply (induction rule: rtranclp_induct)
+  subgoal by simp
+  subgoal using tangle_attractor_step_mono by blast
+  done
+
+lemma tangle_attractor_step_ss: "tangle_attractor_step S S' \<Longrightarrow> fst S' \<subseteq> (fst S \<union> V)"
+  apply (induction rule: tangle_attractor_step.induct)
+  subgoal using V\<^sub>\<alpha>_subset by auto
+  subgoal by simp
+  subgoal using tangles_T player_tangle_in_V by auto
+  done
+
+lemma tangle_attractor_step_rtranclp_ss: "tangle_attractor_step\<^sup>*\<^sup>* S S' \<Longrightarrow> fst S' \<subseteq> (fst S \<union> V)"
+  apply (induction rule: rtranclp_induct)
+  subgoal by simp
+  subgoal using tangle_attractor_step_ss by blast
+  done
+
+lemma fin_tangle_attractor_step: "tangle_attractor_step S S' \<Longrightarrow> finite (fst S) \<Longrightarrow> finite (fst S')"
+  using finite_subset[OF tangle_attractor_step_ss] by blast
+
+lemma fin_tangle_attractor_step_rtranclp: "tangle_attractor_step\<^sup>*\<^sup>* S S' \<Longrightarrow> finite (fst S) \<Longrightarrow> finite (fst S')"
+  using finite_subset[OF tangle_attractor_step_rtranclp_ss] by blast
+
+definition tangle_attractor_step_I :: "'v set \<times> 'v strat \<Rightarrow> bool" where
+  "tangle_attractor_step_I \<equiv> \<lambda>(S,\<sigma>).
    strategy_of V\<^sub>\<alpha> \<sigma> \<and> dom \<sigma> = V\<^sub>\<alpha> \<inter> (S-A) \<and> ran \<sigma> \<subseteq> S \<and>
    induced_subgraph V\<^sub>\<alpha> \<sigma> `` (S-A) \<subseteq> S \<and>
    (\<forall>x\<in>S. \<forall>xs ys. lasso_from_node (induced_subgraph V\<^sub>\<alpha> \<sigma>) x xs ys
       \<longrightarrow> (set (xs@ys) \<inter> A \<noteq> {} \<or> winning_player ys))"
 
-lemma attractor_step_strat_mono: "attractor_step_strat S \<sigma> S' \<sigma>' \<Longrightarrow> S \<subset> S'"
-  by (induction rule: attractor_step_strat.induct) auto
+lemma tangle_attractor_step_I_base: "tangle_attractor_step_I (A,Map.empty)"
+  unfolding tangle_attractor_step_I_def using origin_in_lasso by fastforce
 
-lemma attractor_step_strat_I_base:
-  "attractor_step_strat_I A Map.empty"
-  unfolding attractor_step_strat_I_def
-  using origin_in_lasso by fastforce
-
-lemma attractor_step_strat_I_step:
-  "attractor_step_strat S \<sigma> S' \<sigma>' \<Longrightarrow> A\<subseteq>S \<Longrightarrow> attractor_step_strat_I S \<sigma> \<Longrightarrow> attractor_step_strat_I S' \<sigma>'"
-proof (induction rule: attractor_step_strat.induct)
+lemma tangle_attractor_step_I_step:
+  "tangle_attractor_step S S' \<Longrightarrow> A \<subseteq> fst S \<Longrightarrow> tangle_attractor_step_I S
+   \<Longrightarrow> tangle_attractor_step_I S'"
+proof (induction rule: tangle_attractor_step.induct)
   case (own x S y \<sigma>)
   hence \<sigma>_strat: "strategy_of V\<^sub>\<alpha> \<sigma>" and
-        \<sigma>_dom: "dom \<sigma> = V\<^sub>\<alpha> \<inter> (S-A)" and
-        \<sigma>_ran: "ran \<sigma> \<subseteq> S" and
-        \<sigma>_closed: "induced_subgraph V\<^sub>\<alpha> \<sigma> `` (S-A) \<subseteq> S" and
-        \<sigma>_forces_A_or_wins: "\<forall>x\<in>S. \<forall>xs ys. lasso_from_node (induced_subgraph V\<^sub>\<alpha> \<sigma>) x xs ys
+    \<sigma>_dom: "dom \<sigma> = V\<^sub>\<alpha> \<inter> (S-A)" and
+    \<sigma>_ran: "ran \<sigma> \<subseteq> S" and
+    \<sigma>_closed: "induced_subgraph V\<^sub>\<alpha> \<sigma> `` (S-A) \<subseteq> S" and
+    \<sigma>_forces_A_or_wins: "\<forall>x\<in>S. \<forall>xs ys. lasso_from_node (induced_subgraph V\<^sub>\<alpha> \<sigma>) x xs ys
           \<longrightarrow> (set (xs@ys) \<inter> A \<noteq> {} \<or> winning_player ys)"
-    unfolding attractor_step_strat_I_def by blast+
+    unfolding tangle_attractor_step_I_def by blast+
   let ?S' = "insert x S"
   let ?\<sigma>' = "\<sigma>(x\<mapsto>y)"
 
@@ -162,16 +152,17 @@ proof (induction rule: attractor_step_strat.induct)
   qed
 
   ultimately show ?case
-    unfolding attractor_step_strat_I_def by blast
+    unfolding tangle_attractor_step_I_def by blast
+
 next
   case (opponent x S \<sigma>)
   hence \<sigma>_strat: "strategy_of V\<^sub>\<alpha> \<sigma>" and
-        \<sigma>_dom: "dom \<sigma> = V\<^sub>\<alpha> \<inter> (S-A)" and
-        \<sigma>_ran: "ran \<sigma> \<subseteq> S" and
-        \<sigma>_closed_S: "induced_subgraph V\<^sub>\<alpha> \<sigma> `` (S-A) \<subseteq> S" and
-        \<sigma>_forces_A_or_wins: "\<forall>x\<in>S. \<forall>xs ys. lasso_from_node (induced_subgraph V\<^sub>\<alpha> \<sigma>) x xs ys
+    \<sigma>_dom: "dom \<sigma> = V\<^sub>\<alpha> \<inter> (S-A)" and
+    \<sigma>_ran: "ran \<sigma> \<subseteq> S" and
+    \<sigma>_closed_S: "induced_subgraph V\<^sub>\<alpha> \<sigma> `` (S-A) \<subseteq> S" and
+    \<sigma>_forces_A_or_wins: "\<forall>x\<in>S. \<forall>xs ys. lasso_from_node (induced_subgraph V\<^sub>\<alpha> \<sigma>) x xs ys
           \<longrightarrow> (set (xs@ys) \<inter> A \<noteq> {} \<or> winning_player ys)"
-    unfolding attractor_step_strat_I_def by blast+
+    unfolding tangle_attractor_step_I_def by blast+
   let ?S' = "insert x S"
 
   from \<sigma>_closed_S opponent.hyps(2) have \<sigma>_closed_S': "induced_subgraph V\<^sub>\<alpha> \<sigma> `` (?S'-A) \<subseteq> ?S'"
@@ -180,10 +171,10 @@ next
   have \<sigma>_forces_A_or_wins':
     "\<forall>x\<in>?S'. \<forall>xs ys. lasso_from_node (induced_subgraph V\<^sub>\<alpha> \<sigma>) x xs ys
       \<longrightarrow> (set (xs@ys) \<inter> A \<noteq> {} \<or> winning_player ys)"
-proof (intro ballI allI impI)
+  proof (intro ballI allI impI)
     fix v xs ys
     assume v_in_S': "v \<in> insert x S" and
-           lasso_v_xs_ys: "lasso_from_node (induced_subgraph V\<^sub>\<alpha> \<sigma>) v xs ys"
+      lasso_v_xs_ys: "lasso_from_node (induced_subgraph V\<^sub>\<alpha> \<sigma>) v xs ys"
     from lasso_v_xs_ys obtain v' where
       cycle_v'_ys: "cycle (induced_subgraph V\<^sub>\<alpha> \<sigma>) v' ys"
       unfolding lasso_from_node_def by blast
@@ -234,9 +225,10 @@ proof (intro ballI allI impI)
     qed
     thus "set (xs@ys) \<inter> A \<noteq> {} \<or> winning_player ys" by blast
   qed
-             
+
   from \<sigma>_strat \<sigma>_dom \<sigma>_ran \<sigma>_closed_S' \<sigma>_forces_A_or_wins' opponent.hyps(1) show ?case
-    unfolding attractor_step_strat_I_def by blast
+    unfolding tangle_attractor_step_I_def by blast
+
 next
   case (escape t S \<sigma>' \<sigma>)
   hence \<sigma>_strat: "strategy_of V\<^sub>\<alpha> \<sigma>" and
@@ -245,7 +237,7 @@ next
     \<sigma>_closed_S: "induced_subgraph V\<^sub>\<alpha> \<sigma> `` (S - A) \<subseteq> S" and
     \<sigma>_forces_A_or_wins: "\<forall>x\<in>S. \<forall>xs ys. lasso_from_node (induced_subgraph V\<^sub>\<alpha> \<sigma>) x xs ys
       \<longrightarrow> set (xs @ ys) \<inter> A \<noteq> {} \<or> winning_player ys"
-    unfolding attractor_step_strat_I_def by auto
+    unfolding tangle_attractor_step_I_def by auto
   let ?\<tau> = "(\<sigma>' |` (t-A)) ++ \<sigma>"
   let ?S' = "S\<union>t"
 
@@ -257,11 +249,11 @@ next
     using player_tangle_in_V by auto
 
   from escape.hyps(5) have
-   \<sigma>'_strat: "strategy_of V\<^sub>\<alpha> \<sigma>'" and
-   \<sigma>'_dom: "dom \<sigma>' = t \<inter> V\<^sub>\<alpha>" and
-   \<sigma>'_ran: "ran \<sigma>' \<subseteq> t" and
-   \<sigma>'_strongly_connected_subgraph: "strongly_connected (player_tangle_subgraph t \<sigma>')" and
-   \<sigma>'_winning: "\<forall>v\<in>t. \<forall>xs. cycle (player_tangle_subgraph t \<sigma>') v xs \<longrightarrow> winning_player xs"
+    \<sigma>'_strat: "strategy_of V\<^sub>\<alpha> \<sigma>'" and
+    \<sigma>'_dom: "dom \<sigma>' = t \<inter> V\<^sub>\<alpha>" and
+    \<sigma>'_ran: "ran \<sigma>' \<subseteq> t" and
+    \<sigma>'_strongly_connected_subgraph: "strongly_connected (player_tangle_subgraph t \<sigma>')" and
+    \<sigma>'_winning: "\<forall>v\<in>t. \<forall>xs. cycle (player_tangle_subgraph t \<sigma>') v xs \<longrightarrow> winning_player xs"
     unfolding player_tangle_strat_def Let_def by auto
 
   have \<tau>_strat: "strategy_of V\<^sub>\<alpha> ?\<tau>"
@@ -269,10 +261,10 @@ next
     from \<sigma>'_strat have "strategy_of V\<^sub>\<alpha> (\<sigma>' |` (t-A))"
       unfolding strategy_of_def E_of_strat_def
       apply (simp; safe)
-        subgoal for x y by blast
-        subgoal for x y using restrict_in[of x "t-A" \<sigma>'] by fastforce
+      subgoal for x y by blast
+      subgoal for x y using restrict_in[of x "t-A" \<sigma>'] by fastforce
       done
-      from strategy_of_add_same[OF this \<sigma>_strat] show ?thesis by blast
+    from strategy_of_add_same[OF this \<sigma>_strat] show ?thesis by blast
   qed
 
   from \<sigma>_dom \<sigma>'_dom have \<tau>_dom: "dom ?\<tau> =  V\<^sub>\<alpha> \<inter> (?S' - A)" by auto
@@ -331,10 +323,10 @@ next
         with x_in_S'_min_A have x_in_t_min_A: "x \<in> t-A" by blast
         thus ?thesis
           apply (cases "y\<in>opponent_escapes t")
-            subgoal using escape.hyps(4) by blast
-            subgoal unfolding opponent_escapes_def
-              using notin_\<tau> \<tau>_dom ind_subgraph_edge_in_E[OF x_y_edge] E_in_V
-              by clarsimp blast
+          subgoal using escape.hyps(4) by blast
+          subgoal unfolding opponent_escapes_def
+            using notin_\<tau> \<tau>_dom ind_subgraph_edge_in_E[OF x_y_edge] E_in_V
+            by clarsimp blast
           done
       qed
     qed
@@ -346,7 +338,7 @@ next
   proof (intro ballI allI impI)
     fix v xs ys
     assume v_in_S': "v\<in>?S'" and
-           lasso_v_xs_ys: "lasso_from_node (induced_subgraph V\<^sub>\<alpha> ?\<tau>) v xs ys"
+      lasso_v_xs_ys: "lasso_from_node (induced_subgraph V\<^sub>\<alpha> ?\<tau>) v xs ys"
     from lasso_v_xs_ys obtain v' where
       cycle_v'_ys: "cycle (induced_subgraph V\<^sub>\<alpha> ?\<tau>) v' ys"
       unfolding lasso_from_node_def by blast
@@ -409,517 +401,177 @@ next
   qed
 
   from \<tau>_strat \<tau>_dom \<tau>_ran \<tau>_closed_S' \<tau>_forces_A_or_wins show ?case
-    unfolding attractor_step_strat_I_def by blast
+    unfolding tangle_attractor_step_I_def by blast
 qed
 
-term attractor_step_strat
+lemma tangle_attractor_step_rtranclp_I:
+  "tangle_attractor_step\<^sup>*\<^sup>* S S' \<Longrightarrow> A \<subseteq> fst S \<Longrightarrow> tangle_attractor_step_I S \<Longrightarrow> tangle_attractor_step_I S'"
+  apply (induction rule: rtranclp_induct; simp)
+  using tangle_attractor_step_rtranclp_mono tangle_attractor_step_I_step subset_trans
+  by fast
 
-(** This does not work, how would I be able to do this instead? *)
-
-definition "attractor_step_strat' \<equiv> \<lambda>(s,\<sigma>) (s',\<sigma>'). attractor_step_strat s \<sigma> s' \<sigma>'"
-
-
-
-definition is_player_tangle_attractor_strat :: "('v set \<times> _) \<Rightarrow> bool" where
-  "is_player_tangle_attractor_strat \<equiv> attractor_step_strat'\<^sup>*\<^sup>* (A,Map.empty)"
-  
-term conversep 
-term "conversep attractor_step_strat'"
-
-term finite_psubset
-term inv_image
-
-term "inv_image (finite_psubset) (\<lambda>(s,\<sigma>). V - s)"
-
-
-lemma "wfP (attractor_step_strat'\<inverse>\<inverse>)"  
+lemma tangle_attractor_step_wf: "wfP (tangle_attractor_step\<inverse>\<inverse>)"
   unfolding wfP_def
-  apply (rule wf_subset[of "inv_image (finite_psubset) (\<lambda>(s,\<sigma>). V - s)"])
-  apply simp
-  apply (clarsimp simp: attractor_step_strat'_def)
-  subgoal for s' \<sigma>' s \<sigma>
-    apply (erule attractor_step_strat.cases)
+  apply (rule wf_subset[of "inv_image (finite_psubset) (\<lambda>(s,\<sigma>). V - s)"]; clarsimp)
+  subgoal for S' \<sigma>' S \<sigma>
+    apply (erule tangle_attractor_step.cases)
     subgoal using V\<^sub>\<alpha>_subset by blast
     subgoal by auto
     subgoal using player_tangle_in_V tangles_T by blast
     done
   done
-  
-  
-definition player_tangle_attractor_strat_I :: "'v set \<Rightarrow> bool" where
-  "player_tangle_attractor_strat_I S \<equiv> \<exists>\<sigma>.
-      strategy_of V\<^sub>\<alpha> \<sigma> \<and> dom \<sigma> = V\<^sub>\<alpha> \<inter> (S-A) \<and> ran \<sigma> \<subseteq> S
-    \<and> induced_subgraph V\<^sub>\<alpha> \<sigma> `` (S-A) \<subseteq> S
-    \<and> (\<forall>x\<in>S. \<forall>xs ys. lasso_from_node (induced_subgraph V\<^sub>\<alpha> \<sigma>) x xs ys
-        \<longrightarrow> (set (xs@ys) \<inter> A \<noteq> {} \<or> winning_player ys))"
 
-lemma attractor_step_mono: "attractor_step S S' \<Longrightarrow> S \<subset> S'"
-  by (induction rule: attractor_step.induct) auto
-
-lemma attractor_step_in_S_Un_V: "attractor_step S S' \<Longrightarrow> S' \<subseteq> S \<union> V"
-  apply (induction rule: attractor_step.induct)
-    subgoal using V\<^sub>\<alpha>_subset by auto
-    subgoal by fast
-    subgoal using tangles_T player_tangle_in_V by blast
-  done
-
-lemma attractor_step_in_V: "attractor_step S S' \<Longrightarrow> S \<subseteq> V \<Longrightarrow> S' \<subseteq> V"
-  using attractor_step_in_S_Un_V by blast
-
-lemma "attractor_step S S' \<Longrightarrow> V-S' \<subseteq> V-S"
-  using attractor_step_mono by blast
-
-lemma "attractor_step S S' \<Longrightarrow> S \<subseteq> V \<Longrightarrow> V-S' \<subset> V-S"
-  using attractor_step_mono attractor_step_in_V by blast
-
-lemma player_tangle_attractor_I_base:
-  "player_tangle_attractor_strat_I A"
-  unfolding player_tangle_attractor_strat_I_def
-  apply (rule exI[where x="Map.empty"]; intro conjI; simp)
-  using origin_in_lasso by fastforce
-
-lemma player_tangle_attractor_I_step:
-  "attractor_step S S' \<Longrightarrow> A\<subseteq>S \<Longrightarrow> player_tangle_attractor_strat_I S
-    \<Longrightarrow> player_tangle_attractor_strat_I S'"
-proof (induction rule: attractor_step.induct)
-  case (own x S y)
-  from own.prems obtain \<sigma> where
-    \<sigma>_strat: "strategy_of V\<^sub>\<alpha> \<sigma>" and
-    \<sigma>_dom: "dom \<sigma> = V\<^sub>\<alpha> \<inter> (S-A)" and
-    \<sigma>_ran: "ran \<sigma> \<subseteq> S" and
-    \<sigma>_closed: "induced_subgraph V\<^sub>\<alpha> \<sigma> `` (S-A) \<subseteq> S" and
-    \<sigma>_forces_A_or_wins: "(\<forall>x\<in>S. \<forall>xs ys. lasso_from_node (induced_subgraph V\<^sub>\<alpha> \<sigma>) x xs ys
-        \<longrightarrow> (set (xs@ys) \<inter> A \<noteq> {} \<or> winning_player ys))"
-    unfolding player_tangle_attractor_strat_I_def
-    by auto
-
-  from own.hyps(1,2) have new_strat: "strategy_of V\<^sub>\<alpha> (\<sigma> ++ [x\<mapsto>y])"
-    using strategy_of_add_same[OF \<sigma>_strat strategy_of_map_assign] by blast
-
-  from own.hyps(1) own.prems(1) \<sigma>_dom have new_dom: "dom (\<sigma> ++ [x\<mapsto>y]) = V\<^sub>\<alpha> \<inter> (insert x S - A)"
-    by auto
-
-  from own.hyps(3) \<sigma>_ran have new_ran: "ran (\<sigma> ++ [x\<mapsto>y]) \<subseteq> (insert x S)"
-    unfolding ran_def by auto
-
-  from \<sigma>_closed \<sigma>_ran own.hyps(1)
-  have new_closed_S: "induced_subgraph V\<^sub>\<alpha> (\<sigma> ++ [x\<mapsto>y]) `` (S-A) \<subseteq> S"
-    unfolding induced_subgraph_def E_of_strat_def
-    by (auto split: if_splits simp: ranI)
-  with own.hyps(1,3) have new_closed:
-    "induced_subgraph V\<^sub>\<alpha> (\<sigma> ++ [x\<mapsto>y]) `` (insert x S - A) \<subseteq> insert x S"
-    using ind_subgraph_to_strategy[of _ _ V\<^sub>\<alpha> "\<sigma> ++ [x\<mapsto>y]"] by fastforce
-
-  have new_forces_A_or_wins:
-    "\<forall>v\<in>insert x S. \<forall>xs ys. lasso_from_node (induced_subgraph V\<^sub>\<alpha> (\<sigma> ++ [x\<mapsto>y])) v xs ys
-      \<longrightarrow> set (xs@ys) \<inter> A \<noteq> {} \<or> winning_player ys"
-  proof (intro ballI allI impI)
-    fix v xs ys
-    assume v_in_S': "v \<in> insert x S" and
-           lasso_v_xs_ys: "lasso_from_node (induced_subgraph V\<^sub>\<alpha> (\<sigma> ++ [x\<mapsto>y])) v xs ys"
-    from lasso_v_xs_ys obtain v' where
-      cycle_v'_ys: "cycle (induced_subgraph V\<^sub>\<alpha> (\<sigma> ++ [x\<mapsto>y])) v' ys"
-      unfolding lasso_from_node_def by auto
-
-    have "set (xs@ys) \<inter> A = {} \<Longrightarrow> winning_player ys"
-    proof -
-      assume no_A: "set (xs@ys) \<inter> A = {}"
-      hence xs_no_A: "set xs \<inter> A = {}" and ys_no_A: "set ys \<inter> A = {}" by auto
-      with v_in_S' have v_in_S'_min_A: "v \<in> insert x S - A"
-        using origin_in_lasso[OF lasso_v_xs_ys] by blast
-
-      from lasso_from_node_partially_closed_sets[OF this new_closed xs_no_A ys_no_A lasso_v_xs_ys]
-      have ys_in_S'_min_A: "set ys \<subseteq> insert x S - A" by simp
-      hence y_in_S'_min_A: "v' \<in> insert x S - A"
-        using origin_in_cycle[OF cycle_v'_ys] by auto
-
-      consider (ys_has_x) "x \<in> set ys" | (ys_no_x) "x \<notin> set ys" by blast
-      hence "lasso_from_node (induced_subgraph V\<^sub>\<alpha> \<sigma>) v' [] ys \<and> v'\<in>S" proof cases
-        case ys_has_x
-        from own.hyps(1,2) obtain ys' where
-          cycle_y_ys': "cycle (induced_subgraph V\<^sub>\<alpha> (\<sigma> ++ [x\<mapsto>y])) y ys'" and
-          sets_eq: "set ys' = set ys" and
-          y_in_ys': "y \<in> set ys'"
-          using cycle_intermediate_node[OF cycle_v'_ys ys_has_x]
-          apply clarsimp
-          subgoal for vs'
-            using cycle_D[of "induced_subgraph V\<^sub>\<alpha> (\<sigma> ++ [x\<mapsto>y])" x vs']
-            using ind_subgraph_to_strategy by fastforce
-          done
-
-        from own.hyps(3) sets_eq y_in_ys' ys_no_A have "y \<in> S-A" by blast
-        from cycle_partially_closed_set[OF this new_closed_S cycle_y_ys'] sets_eq ys_no_A
-        have "set ys \<subseteq> S - A" by simp
-        with ys_has_x own.hyps(1) show ?thesis by blast
-      next
-        case ys_no_x
-        from own.hyps(1) have subset:
-          "induced_subgraph V\<^sub>\<alpha> (\<sigma> ++ [x\<mapsto>y]) \<inter> (S-A)\<times>(S-A) \<subseteq> induced_subgraph V\<^sub>\<alpha> \<sigma>"
-          unfolding induced_subgraph_def E_of_strat_def
-          by (auto split: if_splits)
-
-        from ys_no_x ys_in_S'_min_A have ys_in_S_min_A: "set ys \<subseteq> S-A" by blast
-        from subgraph_cycle[OF subset cycle_restr_V[OF cycle_v'_ys this]]
-        have cycle_\<sigma>_v'_ys: " cycle (induced_subgraph V\<^sub>\<alpha> \<sigma>) v' ys " .
-
-        with ys_in_S_min_A have v'_in_S_min_A: "v' \<in> S-A"
-          using origin_in_cycle by fast
-
-        with cycle_\<sigma>_v'_ys show ?thesis by (simp add: cycle_iff_lasso)
-      qed
-      with \<sigma>_forces_A_or_wins ys_no_A show ?thesis by fastforce
-    qed
-    thus "set (xs@ys) \<inter> A \<noteq> {} \<or> winning_player ys" by blast
-  qed
-
-  show ?case
-    unfolding player_tangle_attractor_strat_I_def
-    apply (rule exI[where x="\<sigma> ++ [x\<mapsto>y]"]; intro conjI)
-      subgoal using new_strat .
-      subgoal using new_dom .
-      subgoal using new_ran .
-      subgoal using new_closed .
-      subgoal using new_forces_A_or_wins .
-    done
-
+lemma tangle_attractor_step_rtranclp_induct[consumes 1, case_names base own opponent escape]:
+  assumes tangle_attractor_step_rtranclp: "tangle_attractor_step\<^sup>*\<^sup>* S S'"
+  assumes base: "P S"
+  assumes own: "\<And>x S y \<sigma>. \<lbrakk>x \<in> V\<^sub>\<alpha>-S; (x,y) \<in> E; y \<in> S; P (S,\<sigma>)\<rbrakk> \<Longrightarrow> P (insert x S,\<sigma>(x\<mapsto>y))"
+  assumes opponent: "\<And>x S \<sigma>. \<lbrakk>x \<in> V\<^sub>\<beta>-S; \<forall>y. (x,y) \<in> E \<longrightarrow> y \<in> S; P (S,\<sigma>)\<rbrakk> \<Longrightarrow> P (insert x S,\<sigma>)"
+  assumes escape: "\<And>t S \<sigma>' \<sigma>. \<lbrakk>t \<in> T; t-S \<noteq> {}; opponent_escapes t \<noteq> {}; opponent_escapes t \<subseteq> S;
+                   player_tangle_strat t \<sigma>'; P (S,\<sigma>)\<rbrakk> \<Longrightarrow> P (S\<union>t, \<sigma>' |` (t-A) ++ \<sigma>)"
+  shows "P S'"
+  using tangle_attractor_step_rtranclp base
+proof (induction rule: rtranclp.induct)
+  case (rtrancl_refl S)
+  thus ?case by simp
 next
-  case (opponent x S)
-  from opponent.prems obtain \<sigma> where
-    \<sigma>_strat: "strategy_of V\<^sub>\<alpha> \<sigma>" and
-    \<sigma>_dom: "dom \<sigma> = V\<^sub>\<alpha> \<inter> (S-A)" and
-    \<sigma>_ran: "ran \<sigma> \<subseteq> S" and
-    \<sigma>_closed_S: "induced_subgraph V\<^sub>\<alpha> \<sigma> `` (S-A) \<subseteq> S" and
-    \<sigma>_forces_A_or_wins: "(\<forall>x\<in>S. \<forall>xs ys. lasso_from_node (induced_subgraph V\<^sub>\<alpha> \<sigma>) x xs ys
-        \<longrightarrow> (set (xs@ys) \<inter> A \<noteq> {} \<or> winning_player ys))"
-    unfolding player_tangle_attractor_strat_I_def
-    by auto
-
-  have \<sigma>_closed_S': "induced_subgraph V\<^sub>\<alpha> \<sigma> `` (insert x S - A) \<subseteq> insert x S"
-    using \<sigma>_closed_S opponent.hyps(2) by auto
-
-  have \<sigma>_forces_A_or_wins_S':
-    "\<forall>x\<in>insert x S. \<forall>xs ys. lasso_from_node (induced_subgraph V\<^sub>\<alpha> \<sigma>) x xs ys
-    \<longrightarrow> set (xs @ ys) \<inter> A \<noteq> {} \<or> winning_player ys"
-  proof (intro ballI allI impI)
-    fix v xs ys
-    assume v_in_S': "v \<in> insert x S" and
-           lasso_v_xs_ys: "lasso_from_node (induced_subgraph V\<^sub>\<alpha> \<sigma>) v xs ys"
-    from lasso_v_xs_ys obtain v' where
-      cycle_v'_ys: "cycle (induced_subgraph V\<^sub>\<alpha> \<sigma>) v' ys"
-      unfolding lasso_from_node_def by blast
-
-    have "set (xs@ys) \<inter> A = {} \<Longrightarrow> winning_player ys"
-    proof -
-      assume no_A: "set (xs@ys) \<inter> A = {}"
-      hence xs_no_A: "set xs \<inter> A = {}" and ys_no_A: "set ys \<inter> A = {}" by auto
-      with v_in_S' have "v \<in> insert x S - A"
-        using origin_in_lasso[OF lasso_v_xs_ys] by blast
-
-      from lasso_from_node_partially_closed_sets[OF this \<sigma>_closed_S' xs_no_A ys_no_A lasso_v_xs_ys]
-      have ys_in_S'_min_A: "set ys \<subseteq> insert x S - A" by simp
-      hence v'_in_S'_min_A: "v' \<in> insert x S - A"
-        using origin_in_cycle[OF cycle_v'_ys] by blast
-
-      consider (ys_has_x) "x \<in> set ys" | (ys_no_x) "x \<notin> set ys" by blast
-      hence "lasso_from_node (induced_subgraph V\<^sub>\<alpha> \<sigma>) v' [] ys \<and> v' \<in> S" proof cases
-        case ys_has_x
-        from opponent.hyps(1,2) obtain y ys' where
-          x_y_edge: "(x,y) \<in> induced_subgraph V\<^sub>\<alpha> \<sigma>" and
-          y_in_S: "y \<in> S" and
-          cycle_y_ys': "cycle (induced_subgraph V\<^sub>\<alpha> \<sigma>) y ys'" and
-          sets_eq: "set ys' = set ys" and
-          y_in_ys: "y \<in> set ys"
-          using cycle_intermediate_node[OF cycle_v'_ys ys_has_x]
-          apply clarsimp
-          subgoal for vs'
-            using cycle_D[of "induced_subgraph V\<^sub>\<alpha> \<sigma>" x vs']
-            using ind_subgraph_to_strategy by blast
-          done
-
-        from y_in_S y_in_ys ys_no_A have y_in_S_min_A: "y \<in> S-A" by blast
-        from cycle_partially_closed_set[OF this \<sigma>_closed_S cycle_y_ys'] sets_eq ys_no_A
-        have "set ys \<subseteq> S-A" by auto
-        hence "v' \<in> S"
-          using origin_in_cycle[OF cycle_v'_ys] by blast
-
-        with cycle_v'_ys show ?thesis by (simp add: cycle_iff_lasso)
-      next
-        case ys_no_x
-        with ys_in_S'_min_A have ys_in_S_min_A: "set ys \<subseteq> S-A" by blast
-        with origin_in_cycle[OF cycle_v'_ys] have v'_in_S_min_A: "v' \<in> S-A" by blast
-        with cycle_v'_ys show ?thesis by (simp add: cycle_iff_lasso)
-      qed
-
-      with \<sigma>_forces_A_or_wins no_A show ?thesis by fastforce
-    qed
-    thus "set (xs@ys) \<inter> A \<noteq> {} \<or> winning_player ys" by blast
-  qed
-
+  case (rtrancl_into_rtrancl S S' S'')
+  from this(2) this(3)[OF this(4)]
   show ?case
-    unfolding player_tangle_attractor_strat_I_def
-    apply (rule exI[where x="\<sigma>"]; intro conjI)
-      subgoal using \<sigma>_strat .
-      subgoal using \<sigma>_dom opponent.hyps(1) by force
-      subgoal using \<sigma>_ran by auto
-      subgoal using \<sigma>_closed_S' .
-      subgoal using \<sigma>_forces_A_or_wins_S' .
-    done
-
-next
-  case (escape t S)
-  from escape.prems obtain \<sigma> where
-    \<sigma>_strat: "strategy_of V\<^sub>\<alpha> \<sigma>" and
-    \<sigma>_dom: "dom \<sigma> = V\<^sub>\<alpha> \<inter> (S - A)" and
-    \<sigma>_ran: "ran \<sigma> \<subseteq> S" and
-    \<sigma>_closed_S: "induced_subgraph V\<^sub>\<alpha> \<sigma> `` (S - A) \<subseteq> S" and
-    \<sigma>_forces_A_or_wins: "\<forall>x\<in>S. \<forall>xs ys. lasso_from_node (induced_subgraph V\<^sub>\<alpha> \<sigma>) x xs ys
-      \<longrightarrow> set (xs @ ys) \<inter> A \<noteq> {} \<or> winning_player ys"
-    unfolding player_tangle_attractor_strat_I_def by auto
-
-  from escape.hyps(1) have t_tangle: "player_tangle t" using tangles_T by simp
-
-  from t_tangle have
-    t_notempty: "t \<noteq> {}" and
-    t_in_V: "t \<subseteq> V"
-    using player_tangle_in_V by auto
-
-  from t_tangle obtain \<sigma>' where
-   \<sigma>'_strat: "strategy_of V\<^sub>\<alpha> \<sigma>'" and
-   \<sigma>'_dom: "dom \<sigma>' = t \<inter> V\<^sub>\<alpha>" and
-   \<sigma>'_ran: "ran \<sigma>' \<subseteq> t" and
-   \<sigma>'_strongly_connected_subgraph: "strongly_connected (player_tangle_subgraph t \<sigma>')" and
-   \<sigma>'_winning: "\<forall>v\<in>t. \<forall>xs. cycle (player_tangle_subgraph t \<sigma>') v xs \<longrightarrow> winning_player xs"
-    unfolding player_tangle_def player_tangle_strat_def Let_def by auto
-
-  define \<tau> where "\<tau> = (\<sigma>' |` (t-A)) ++ \<sigma>"
-  have \<tau>_strat: "strategy_of V\<^sub>\<alpha> \<tau>"
-  proof -
-    from \<sigma>'_strat have "strategy_of V\<^sub>\<alpha> (\<sigma>' |` (t-A))"
-      unfolding strategy_of_def E_of_strat_def
-      apply (simp; safe)
-        subgoal for x y by blast
-        subgoal for x y using restrict_in[of x "t-A" \<sigma>'] by fastforce
-      done
-      from strategy_of_add_same[OF this \<sigma>_strat] show ?thesis
-        unfolding \<tau>_def by blast
-  qed
-
-  from \<sigma>_dom \<sigma>'_dom have \<tau>_dom: "dom \<tau> =  V\<^sub>\<alpha> \<inter> (S \<union> t - A)"
-    unfolding \<tau>_def by auto
-
-  have \<tau>_ran: "ran \<tau> \<subseteq> S\<union>t"
-  proof -
-    have "ran (\<sigma>' |` (t-A)) \<subseteq> t"
-      using subsetD[OF \<sigma>'_ran] ran_restrictD[of _ \<sigma>' "t-A"] ranI by fast
-    with \<sigma>_ran show ?thesis
-      unfolding \<tau>_def ran_def by blast
-  qed
-
-  have \<tau>_closed_S: "induced_subgraph V\<^sub>\<alpha> \<tau> `` (S-A) \<subseteq> S"
-  proof (rule subsetI)
-    fix y assume y_succ: "y\<in>induced_subgraph V\<^sub>\<alpha> \<tau> `` (S-A)"
-    then obtain x where
-      x_y_edge: "(x,y)\<in>induced_subgraph V\<^sub>\<alpha> \<tau>" and
-      x_in_S_min_A: "x\<in>S-A"
-      by blast
-    consider (in_\<tau>) "x \<in> dom \<tau>" | (notin_\<tau>) "x \<notin> dom \<tau>" by blast
-    thus "y \<in> S" proof cases
-      case in_\<tau>
-      with \<tau>_dom have x_in_V\<^sub>\<alpha>: "x \<in> V\<^sub>\<alpha>" by simp
-      from ind_subgraph_to_strategy[OF x_y_edge x_in_V\<^sub>\<alpha>] have \<tau>_x_y: "\<tau> x = Some y" .
-
-      from x_in_V\<^sub>\<alpha> \<tau>_x_y \<sigma>_dom \<sigma>_ran x_in_S_min_A show ?thesis
-        unfolding \<tau>_def by (simp add: map_add_dom_app_simps(1) ranI subsetD)
-    next
-      case notin_\<tau>
-      with x_y_edge \<tau>_dom x_in_S_min_A
-      have x_y_edge_\<sigma>: "(x,y)\<in>induced_subgraph V\<^sub>\<alpha> \<sigma>"
-        using ind_subgraph_notin_dom by auto
-      with \<sigma>_closed_S x_in_S_min_A show ?thesis by blast
-    qed
-  qed
-
-  have \<tau>_closed_S': "induced_subgraph V\<^sub>\<alpha> \<tau> `` (S\<union>t-A) \<subseteq> S\<union>t"
-  proof (rule subsetI)
-    fix y assume y_succ: "y\<in>induced_subgraph V\<^sub>\<alpha> \<tau> `` (S\<union>t-A)"
-    then obtain x where
-      x_y_edge: "(x,y)\<in>induced_subgraph V\<^sub>\<alpha> \<tau>" and
-      x_in_S'_min_A: "x\<in>S\<union>t-A"
-      by blast
-
-    consider (in_\<tau>) "x \<in> dom \<tau>" | (notin_\<tau>) "x \<notin> dom \<tau>" by blast
-    thus "y\<in>S\<union>t" proof cases
-      case in_\<tau> with \<tau>_dom \<tau>_ran show ?thesis
-        using ind_subgraph_edge_dst[OF x_y_edge] by blast
-    next
-      case notin_\<tau>
-      consider (in_S_min_A) "x \<in> S-A" | (notin_S_min_A) "x \<notin> S-A" by blast
-      thus ?thesis proof cases
-        case in_S_min_A with x_y_edge \<tau>_closed_S show ?thesis by blast
-      next
-        case notin_S_min_A
-        with x_in_S'_min_A have x_in_t_min_A: "x \<in> t-A" by blast
-        thus ?thesis
-          apply (cases "y\<in>opponent_escapes t")
-            subgoal using escape.hyps(4) by blast
-            subgoal unfolding opponent_escapes_def
-              using notin_\<tau> \<tau>_dom ind_subgraph_edge_in_E[OF x_y_edge] E_in_V
-              by blast
-          done
-      qed
-    qed
-  qed
-
-  have \<tau>_forces_A_or_wins:
-    "\<forall>x\<in>S \<union> t. \<forall>xs ys. lasso_from_node (induced_subgraph V\<^sub>\<alpha> \<tau>) x xs ys
-      \<longrightarrow> set (xs @ ys) \<inter> A \<noteq> {} \<or> winning_player ys"
-  proof (intro ballI allI impI)
-    fix v xs ys
-    assume v_in_S': "v\<in>S\<union>t" and
-           lasso_v_xs_ys: "lasso_from_node (induced_subgraph V\<^sub>\<alpha> \<tau>) v xs ys"
-    from lasso_v_xs_ys obtain v' where
-      cycle_v'_ys: "cycle (induced_subgraph V\<^sub>\<alpha> \<tau>) v' ys"
-      unfolding lasso_from_node_def by blast
-
-    have "set (xs@ys) \<inter> A = {} \<Longrightarrow> winning_player ys"
-    proof -
-      assume no_A: "set (xs@ys) \<inter> A = {}"
-      hence xs_no_A: "set xs \<inter> A = {}" and ys_no_A: "set ys \<inter> A = {}" by auto
-      with v_in_S' have "v\<in>(S\<union>t)-A"
-        using origin_in_lasso[OF lasso_v_xs_ys] by blast
-
-      from lasso_from_node_partially_closed_sets[OF this \<tau>_closed_S' xs_no_A ys_no_A lasso_v_xs_ys]
-      have ys_in_S'_min_A: "set ys \<subseteq> (S\<union>t)-A" by simp
-      hence v'_in_S'_min_A: "v' \<in> (S\<union>t)-A"
-        using origin_in_cycle[OF cycle_v'_ys] by blast
-
-      consider (ys_has_S) "set ys \<inter> S \<noteq> {}" | (ys_no_S) "set ys \<inter> S = {}" by blast
-      thus ?thesis proof cases
-        (** In this case, the cycle must be entirely contained in S because S is closed under
-            \<tau>. That also means it is won because under \<sigma>, all plays that do not go through A
-            are winning. *)
-        case ys_has_S
-        with ys_no_A obtain y ys' where
-          y_in_S_min_A: "y \<in> S-A" and
-          sets_eq: "set ys' = set ys" and
-          ys'_no_A: "set ys' \<inter> A = {}" and
-          cycle_y_ys': "cycle (induced_subgraph V\<^sub>\<alpha> \<tau>) y ys'"
-          using cycle_intermediate_node[OF cycle_v'_ys] by fastforce
-
-        from cycle_partially_closed_set[OF y_in_S_min_A \<tau>_closed_S cycle_y_ys' ys'_no_A] sets_eq
-        have ys_in_S_min_A: "set ys \<subseteq> S-A" by blast
-        hence v'_in_S: "v' \<in> S" using origin_in_cycle[OF cycle_v'_ys] by blast
-
-        from \<sigma>_dom have subset: "induced_subgraph V\<^sub>\<alpha> \<tau> \<inter> (S-A)\<times>(S-A) \<subseteq> induced_subgraph V\<^sub>\<alpha> \<sigma>"
-          unfolding \<tau>_def induced_subgraph_def E_of_strat_def by auto
-
-        from subgraph_cycle[OF subset cycle_restr_V[OF cycle_v'_ys ys_in_S_min_A]]
-        have "lasso_from_node (induced_subgraph V\<^sub>\<alpha> \<sigma>) v' [] ys"
-          by (simp add: cycle_iff_loop loop_impl_lasso)
-
-        with \<sigma>_forces_A_or_wins v'_in_S no_A show ?thesis by fastforce
-      next
-        case ys_no_S
-        with ys_in_S'_min_A have ys_in_t_min_S_min_A: "set ys \<subseteq> t-S-A" by blast
-        hence v'_in_t: "v'\<in>t" using origin_in_cycle[OF cycle_v'_ys] by blast
-
-        from \<sigma>_ran t_in_V have subset:
-          "induced_subgraph V\<^sub>\<alpha> \<tau> \<inter> (t-S-A)\<times>(t-S-A) \<subseteq> player_tangle_subgraph t \<sigma>' \<inter> (t-S-A)\<times>(t-S-A)"
-          unfolding \<tau>_def induced_subgraph_def player_tangle_subgraph_def E_of_strat_def
-          using ind_subgraph_edge_dst[of _ _ V\<^sub>\<alpha> \<sigma>] strategy_to_ind_subgraph[of \<sigma> _ _ V\<^sub>\<alpha>]
-          by fastforce
-
-        from subgraph_cycle[OF subset cycle_restr_V[OF cycle_v'_ys ys_in_t_min_S_min_A]]
-        have "cycle (player_tangle_subgraph t \<sigma>') v' ys" using restr_V_cycle by fast
-
-        with \<sigma>'_winning v'_in_t show ?thesis by blast
-      qed
-    qed
-    thus "set (xs@ys) \<inter> A \<noteq> {} \<or> winning_player ys" by blast
-  qed
-
-  show ?case
-    unfolding player_tangle_attractor_strat_I_def
-    apply (rule exI[where x="\<tau>"]; intro conjI)
-      subgoal using \<tau>_strat .
-      subgoal using \<tau>_dom .
-      subgoal using \<tau>_ran .
-      subgoal using \<tau>_closed_S' .
-      subgoal using \<tau>_forces_A_or_wins .
+    apply (induction rule: tangle_attractor_step.induct)
+    subgoal using own by simp
+    subgoal using opponent by simp
+    subgoal using escape by simp
     done
 qed
 
-definition is_player_tangle_attractor :: "'v set \<Rightarrow> bool" where
-  "is_player_tangle_attractor \<equiv> attractor_step\<^sup>*\<^sup>* A"
+(** Correctness check for the induction lemma *)
+lemma "tangle_attractor_step\<^sup>*\<^sup>* S S' \<Longrightarrow> finite (fst S) \<Longrightarrow> finite (fst S')"
+  apply (induction rule: tangle_attractor_step_rtranclp_induct)
+  subgoal by simp
+  subgoal by simp
+  subgoal by simp
+  subgoal using tangles_T fin_player_tangle by simp
+  done
 
-lemma attractor_step_rtranclp_subset: "attractor_step\<^sup>*\<^sup>* S S' \<Longrightarrow> S \<subseteq> S'"
-  apply (induction rule: rtranclp_induct)
-  using attractor_step_mono by blast+
+definition player_tangle_attractor :: "'v set \<Rightarrow> 'v strat \<Rightarrow> bool" where
+  "player_tangle_attractor X \<sigma> \<equiv> tangle_attractor_step\<^sup>*\<^sup>* (A,Map.empty) (X,\<sigma>)"
 
-lemma attractor_step_rtrancl:
-  "attractor_step\<^sup>*\<^sup>* S S' \<Longrightarrow> A \<subseteq> S \<Longrightarrow> player_tangle_attractor_strat_I S
-    \<Longrightarrow> player_tangle_attractor_strat_I S'"
-  apply (induction rule: rtranclp_induct; simp)
-  using attractor_step_rtranclp_subset player_tangle_attractor_I_step by fast
+lemma player_tangle_attractor_induct[consumes 1, case_names base own opponent escape]:
+  assumes attr: "player_tangle_attractor X \<sigma>"
+  assumes base: "P A Map.empty"
+  assumes own: "\<And>x S y \<sigma>. \<lbrakk>x \<in> V\<^sub>\<alpha>-S; (x,y) \<in> E; y \<in> S; P S \<sigma>\<rbrakk> \<Longrightarrow> P (insert x S) (\<sigma>(x\<mapsto>y))"
+  assumes opponent: "\<And>x S \<sigma>. \<lbrakk>x \<in> V\<^sub>\<beta> - S; \<forall>y. (x,y) \<in> E \<longrightarrow> y \<in> S; P S \<sigma>\<rbrakk> \<Longrightarrow> P (insert x S) \<sigma>"
+  assumes escape: "\<And>t S \<sigma>' \<sigma>. \<lbrakk>t \<in> T; t-S \<noteq> {}; opponent_escapes t \<noteq> {}; opponent_escapes t \<subseteq> S;
+                   player_tangle_strat t \<sigma>'; P S \<sigma>\<rbrakk> \<Longrightarrow> P (S\<union>t) (\<sigma>' |` (t-A) ++ \<sigma>)"
+  shows "P X \<sigma>"
+proof -
+  define P' :: "'v set \<times> 'v strat \<Rightarrow> bool" where "P' \<equiv> \<lambda>(a,b). P a b"
+  hence base': "P' (A,Map.empty)" and
+        own': "\<And>x S y \<sigma>. \<lbrakk>x \<in> V\<^sub>\<alpha>-S; (x,y) \<in> E; y \<in> S; P' (S,\<sigma>)\<rbrakk> \<Longrightarrow> P' (insert x S,\<sigma>(x\<mapsto>y))" and
+        opponent': "\<And>x S \<sigma>. \<lbrakk>x \<in> V\<^sub>\<beta>-S; \<forall>y. (x,y) \<in> E \<longrightarrow> y \<in> S; P' (S,\<sigma>)\<rbrakk> \<Longrightarrow> P' (insert x S,\<sigma>)" and
+        escape': "\<And>t S \<sigma>' \<sigma>. \<lbrakk>t \<in> T; t-S \<noteq> {}; opponent_escapes t \<noteq> {}; opponent_escapes t \<subseteq> S;
+                  player_tangle_strat t \<sigma>'; P' (S,\<sigma>)\<rbrakk> \<Longrightarrow> P' (S\<union>t,\<sigma>' |` (t-A) ++ \<sigma>)"
+    using base own opponent escape by auto
+  from attr base'
+  have "P' (X,\<sigma>)"
+    unfolding player_tangle_attractor_def
+    apply (induction rule: tangle_attractor_step_rtranclp_induct)
+    using own' opponent' escape' by auto
+  thus ?thesis
+    unfolding P'_def by simp
+qed
+
+lemma A_in_player_tangle_attractor: "player_tangle_attractor U \<sigma> \<Longrightarrow> A \<subseteq> U"
+  unfolding player_tangle_attractor_def
+  using tangle_attractor_step_rtranclp_mono by fastforce
+
+lemma player_tangle_attractor_ss: "player_tangle_attractor U \<sigma> \<Longrightarrow> U \<subseteq> A \<union> V"
+  unfolding player_tangle_attractor_def
+  using tangle_attractor_step_rtranclp_ss by fastforce
+
+lemma fin_player_tangle_attractor: "player_tangle_attractor U \<sigma> \<Longrightarrow> finite A \<Longrightarrow> finite U"
+  using finite_subset[OF player_tangle_attractor_ss] by blast
+
+lemma player_tangle_attractor_strat: "player_tangle_attractor U \<sigma> \<Longrightarrow>
+      strategy_of V\<^sub>\<alpha> \<sigma> \<and> dom \<sigma> = V\<^sub>\<alpha> \<inter> (U-A) \<and> ran \<sigma> \<subseteq> U \<and>
+      induced_subgraph V\<^sub>\<alpha> \<sigma> `` (U-A) \<subseteq> U \<and>
+      (\<forall>x\<in>U. \<forall>xs ys. lasso_from_node (induced_subgraph V\<^sub>\<alpha> \<sigma>) x xs ys
+        \<longrightarrow> set (xs @ ys) \<inter> A \<noteq> {} \<or> winning_player ys)"
+  using tangle_attractor_step_I_base tangle_attractor_step_rtranclp_I
+  unfolding player_tangle_attractor_def tangle_attractor_step_I_def
+  by clarsimp
 end (** End of context with fixed A *)
-
-lemma is_player_tangle_attractor_I_holds:
-  "is_player_tangle_attractor A S \<Longrightarrow> player_tangle_attractor_strat_I A S"
-  unfolding is_player_tangle_attractor_def
-  using player_tangle_attractor_I_base attractor_step_rtrancl by blast
-
-lemma player_tangle_attractor_is_valid:
-  "is_player_tangle_attractor A (player_tangle_attractor A)"
-  unfolding is_player_tangle_attractor_def
-  sorry ,xxx sorry (** I do not know how to prove this right now. *)
-
-lemma player_tangle_attractor_strat: "\<exists>\<sigma>. player_tangle_attractor_strat \<sigma> A"
-  using player_tangle_attractor_is_valid is_player_tangle_attractor_I_holds
-  unfolding player_tangle_attractor_strat_I_def player_tangle_attractor_strat_def
-  by simp
 
 
 subsection \<open>\<alpha>-maximal Regions\<close>
 (** A region is \<alpha>-maximal if it equals its tangle attractor. *)
 definition player_\<alpha>_max :: "'v set \<Rightarrow> bool" where
-  "player_\<alpha>_max A \<equiv> A = player_tangle_attractor A"
+  "player_\<alpha>_max A \<equiv> player_tangle_attractor A A Map.empty"
 
-lemma player_\<alpha>_max_empty_strat: "player_\<alpha>_max A \<Longrightarrow> player_tangle_attractor_strat Map.empty A"
-  unfolding player_\<alpha>_max_def player_tangle_attractor_strat_def
-  using origin_in_lasso by fastforce
+lemma attracted_region_is_player_\<alpha>_max: "player_tangle_attractor A U \<sigma> \<Longrightarrow> player_\<alpha>_max U"
+  unfolding player_\<alpha>_max_def
+  apply (induction rule: player_tangle_attractor_induct)
+  subgoal unfolding player_tangle_attractor_def by blast
+  subgoal unfolding player_tangle_attractor_def by blast
+  subgoal unfolding player_tangle_attractor_def by blast
+  subgoal unfolding player_tangle_attractor_def by blast
+  done
 
 end (** End of context with fixed T *)
+
+(** We need this version of the induction lemma so we can supply the properties of T without losing
+    our case names. *)
+lemma player_tangle_attractor_induct'[consumes 3, case_names base own opponent escape]:
+  assumes attr: "player_tangle_attractor T A X \<sigma>"
+  assumes tangles_T: "\<forall>t\<in>T. player_tangle t"
+  assumes fin_T: "finite T"
+  assumes base: "P A Map.empty"
+  assumes own: "\<And>x S y \<sigma>. \<lbrakk>x \<in> V\<^sub>\<alpha>-S; (x,y) \<in> E; y \<in> S; P S \<sigma>\<rbrakk> \<Longrightarrow> P (insert x S) (\<sigma>(x\<mapsto>y))"
+  assumes opponent: "\<And>x S \<sigma>. \<lbrakk>x \<in> V\<^sub>\<beta> - S; \<forall>y. (x,y) \<in> E \<longrightarrow> y \<in> S; P S \<sigma>\<rbrakk> \<Longrightarrow> P (insert x S) \<sigma>"
+  assumes escape: "\<And>t S \<sigma>' \<sigma>. \<lbrakk>t \<in> T; t-S \<noteq> {}; opponent_escapes t \<noteq> {}; opponent_escapes t \<subseteq> S;
+                   player_tangle_strat t \<sigma>'; P S \<sigma>\<rbrakk> \<Longrightarrow> P (S\<union>t) (\<sigma>' |` (t-A) ++ \<sigma>)"
+  shows "P X \<sigma>"
+  using player_tangle_attractor_induct[OF tangles_T fin_T attr] base own opponent escape by blast
+
 end (** End of context player_paritygame *)
 
 section \<open>Tangle Attractors for Specific Players\<close>
 context paritygame begin
 
-fun tangle_attractor :: "player \<Rightarrow> 'v set set  \<Rightarrow> 'v set \<Rightarrow> 'v set" where
-  "tangle_attractor EVEN T = P0.player_tangle_attractor T"
-| "tangle_attractor ODD T = P1.player_tangle_attractor T"
+fun tangle_attractor :: "player \<Rightarrow> 'v set set \<Rightarrow> 'v set \<Rightarrow> 'v set \<Rightarrow> 'v strat \<Rightarrow> bool" where
+  "tangle_attractor EVEN = P0.player_tangle_attractor"
+| "tangle_attractor ODD = P1.player_tangle_attractor"
 
-fun tangle_attractor_strat :: "player \<Rightarrow> 'v set set \<Rightarrow> 'v strat \<Rightarrow> 'v set \<Rightarrow> bool" where
-  "tangle_attractor_strat EVEN T = P0.player_tangle_attractor_strat T"
-| "tangle_attractor_strat ODD T = P1.player_tangle_attractor_strat T"
+lemma A_in_tangle_attractor:
+  assumes tangles_T: "\<forall>t\<in>T. tangle \<alpha> t"
+  assumes fin_T: "finite T"
+  shows "tangle_attractor \<alpha> T A U \<sigma> \<Longrightarrow> A \<subseteq> U"
+  using assms P0.A_in_player_tangle_attractor P1.A_in_player_tangle_attractor
+  by (cases \<alpha>; simp)
+
+lemma tangle_attractor_ss:
+  assumes tangles_T: "\<forall>t\<in>T. tangle \<alpha> t"
+  assumes fin_T: "finite T"
+  shows "tangle_attractor \<alpha> T A U \<sigma> \<Longrightarrow> U \<subseteq> A \<union> V"
+  using assms P0.player_tangle_attractor_ss P1.player_tangle_attractor_ss
+  by (cases \<alpha>; simp)
 
 lemma tangle_attractor_strat:
-  assumes "\<forall>t\<in>T. tangle \<alpha> t"
-  assumes "finite T"
-  shows "\<exists>\<sigma>. tangle_attractor_strat \<alpha> T \<sigma> A"
+  assumes tangles_T: "\<forall>t\<in>T. tangle \<alpha> t"
+  assumes fin_T: "finite T"
+  shows "tangle_attractor \<alpha> T A U \<sigma> \<Longrightarrow>
+         strategy_of_player \<alpha> \<sigma> \<and> dom \<sigma> = V_player \<alpha> \<inter> (U-A) \<and> ran \<sigma> \<subseteq> U \<and>
+         induced_subgraph (V_player \<alpha>) \<sigma> `` (U-A) \<subseteq> U \<and>
+         (\<forall>x\<in>U. \<forall>xs ys. lasso_from_node (induced_subgraph (V_player \<alpha>) \<sigma>) x xs ys
+            \<longrightarrow> set (xs @ ys) \<inter> A \<noteq> {} \<or> player_wins_list \<alpha> ys)"
+  unfolding strategy_of_player_def
   using assms P0.player_tangle_attractor_strat P1.player_tangle_attractor_strat
   by (cases \<alpha>; simp add: V\<^sub>1_def)
 
+subsection \<open>\<alpha>-maximal regions\<close>
 fun \<alpha>_max :: "player \<Rightarrow> 'v set set \<Rightarrow> 'v set \<Rightarrow> bool" where
-  "\<alpha>_max EVEN T = P0.player_\<alpha>_max T"
-| "\<alpha>_max ODD T = P1.player_\<alpha>_max T"
-
-lemma \<alpha>_max_empty_strat:
-  assumes "\<forall>t\<in>T. tangle \<alpha> t"
-  assumes "finite T"
-  shows "\<alpha>_max \<alpha> T A \<Longrightarrow> tangle_attractor_strat \<alpha> T Map.empty A"
-  using assms P0.player_\<alpha>_max_empty_strat P1.player_\<alpha>_max_empty_strat
-  by (cases \<alpha>; simp)
-
+  "\<alpha>_max EVEN = P0.player_\<alpha>_max"
+| "\<alpha>_max ODD = P1.player_\<alpha>_max"
 end (** End of context paritygame *)
 
 end
