TangleLearning.thy
@@ -12,92 +12,32 @@ lemma van_dijk_1_player: *)
 
 (** Lemma 2:
     all plays bound by the tangle attractor strategy \<sigma> that stay in that tangle attractor
-    to a region consisting only of vertices of the highest priority, won by \<alpha>, are won by \<alpha>. *)
+    to a region consisting only of vertices of the highest priority, won by \<alpha>, are won by \<alpha>.
+
+    In the search-algorithm, we talk about a region R in the graph that A is inside of, with A
+    containing all top priority nodes in R. However, it is easier to prove this assuming we take
+    the highest priorities in V. For a final proof then, we have to show that any R is a valid
+    subgame.
+
+    Note that we also assume that all tangles in T belong to the player. The final proof will have
+    to filter its T based on which player owns the tangles to use this lemma. *)
 lemma van_dijk_2_player:
-  assumes tangles_T: "\<forall>t\<in>T. player_tangle t"
-  assumes fin_T: "finite T"
-  assumes R_in_V: "R \<subseteq> V"
-  assumes top_pr_p: "p = pr_set R"
-  assumes winning_p: "winningP p"
-  assumes A_def: "A = {v. v\<in>R \<and> pr v = p}"
-  assumes \<sigma>_attr_strat: "player_tangle_attractor_strat T \<sigma> A"
-  shows "\<forall>v\<in>player_tangle_attractor T A.
-                \<forall>xs ys. lasso_from_node (induced_subgraph V\<^sub>\<alpha> \<sigma> \<inter> (player_tangle_attractor T A \<times> player_tangle_attractor T A)) v xs ys \<longrightarrow> winning_player ys"
-proof (intro ballI allI impI)
-  let ?Z = "player_tangle_attractor T A"
-  let ?restr_subgraph = "induced_subgraph V\<^sub>\<alpha> \<sigma> \<inter> (?Z \<times> ?Z)"
-  fix v xs ys
-  assume v_in_Z: "v \<in> ?Z" and
-         lasso_restr_Z_v_xs_ys: "lasso_from_node ?restr_subgraph v xs ys"
-
-  from tangles_T fin_T \<sigma>_attr_strat have
-    \<sigma>_strat: "strategy_of V\<^sub>\<alpha> \<sigma>" and
-    \<sigma>_dom: "dom \<sigma> = V\<^sub>\<alpha> \<inter> (?Z - A)" and
-    \<sigma>_ran: "ran \<sigma> \<subseteq> ?Z" and
-    \<sigma>_closed: "induced_subgraph V\<^sub>\<alpha> \<sigma> `` (?Z - A) \<subseteq> ?Z" and
-    \<sigma>_forces_A_or_wins: "\<forall>x\<in>?Z. \<forall>xs ys. lasso_from_node (induced_subgraph V\<^sub>\<alpha> \<sigma>) x xs ys
-      \<longrightarrow> set (xs @ ys) \<inter> A \<noteq> {} \<or> winning_player ys"
-    by (simp add: player_tangle_attractor_strat_def)+
-
-  from restr_V_lasso[OF lasso_restr_Z_v_xs_ys]
-  have xs_in_Z: "set xs \<subseteq> ?Z" and
-       ys_in_Z: "set ys \<subseteq> ?Z" and
-       lasso_v_xs_ys: "lasso_from_node (induced_subgraph V\<^sub>\<alpha> \<sigma>) v xs ys"
-    by blast+
-
-  show "winning_player ys" proof(rule ccontr)
-    assume not_winning: "winning_opponent ys"
-    with \<sigma>_forces_A_or_wins lasso_v_xs_ys v_in_Z
-    have A_in_xs_ys: "set (xs@ys) \<inter> A \<noteq> {}" by blast
-
-    consider "set ys \<inter> A \<noteq> {}" | "set ys \<inter> A = {}" by blast
-    hence "winning_player ys" proof cases
-      case 1
-      (** Because A consists of nodes of the highest priority in R, it should always have
-          the winning priority, but this current lemma formulation does not specify that the
-          tangle attractor remains in R.
-          Possible solution: forget about R, take the highest priority in V instead.
-          For an actual proof of the algorithm, we just need to limit to a subgame R.
-          See below! *)
-      then show ?thesis sorry
-    next
-      case 2
-      from lasso_from_node_loop[OF lasso_v_xs_ys] obtain y where
-         lasso_y_ys: "lasso_from_node (induced_subgraph V\<^sub>\<alpha> \<sigma>) y [] ys" and
-         y_in_ys: "y \<in> set ys" by blast
-      with ys_in_Z have y_in_Z: "y \<in> ?Z" by blast
-
-      with \<sigma>_forces_A_or_wins lasso_y_ys 2 show ?thesis by auto
-    qed
-
-    show "False" sorry
-  qed
-qed
-
-(** We can rephrase the second lemma to ignore the region R and instead use a whole game. This would
-    work in the final proof because R is created either from the whole game, or by subtracting an
-    attractor from the previous region, which means it is always a valid subgame. *)
-lemma van_dijk_2_player':
   assumes tangles_T: "\<forall>t\<in>T. player_tangle t"
   assumes fin_T: "finite T"
   assumes winning_top_p: "winningP (pr_set V)"
   assumes A_def: "A = {v. v\<in>V \<and> pr v = pr_set V}"
-  assumes \<sigma>_attr_strat: "player_tangle_attractor_strat T \<sigma> A"
-  shows "\<forall>v\<in>player_tangle_attractor T A.
-          \<forall>xs ys. lasso_from_node (induced_subgraph V\<^sub>\<alpha> \<sigma> \<inter> (player_tangle_attractor T A \<times> player_tangle_attractor T A)) v xs ys
-            \<longrightarrow> winning_player ys"
+  assumes attr: "player_tangle_attractor T A Z \<sigma>"
+  shows "\<forall>v\<in>Z. \<forall>xs ys.
+          lasso_from_node (induced_subgraph V\<^sub>\<alpha> \<sigma> \<inter> (Z \<times> Z)) v xs ys \<longrightarrow> winning_player ys"
 proof (intro ballI allI impI)
-  let ?Z = "player_tangle_attractor T A"
-  from player_tangle_attractor_ss[OF tangles_T fin_T, of A] A_def
-  have Z_in_V: "?Z \<subseteq> V" by blast
-  let ?restr_subgraph = "induced_subgraph V\<^sub>\<alpha> \<sigma> \<inter> (?Z \<times> ?Z)"
-
+  let ?restr_subgraph = "induced_subgraph V\<^sub>\<alpha> \<sigma> \<inter> (Z \<times> Z)"
   fix v xs ys
-  assume v_in_Z: "v \<in> ?Z" and
-         lasso_restr_Z_v_xs_ys: "lasso_from_node ?restr_subgraph v xs ys"
+  assume v_in_Z: "v\<in>Z" and lasso_restr_v_xs_ys: "lasso_from_node ?restr_subgraph v xs ys"
+  from player_tangle_attractor_ss[OF tangles_T fin_T attr] A_def
+  have Z_in_V: "Z \<subseteq> V" by blast
 
-  from restr_V_lasso[OF lasso_restr_Z_v_xs_ys] have
-    ys_in_Z: "set ys \<subseteq> ?Z" and
+  from restr_V_lasso[OF lasso_restr_v_xs_ys] have
+    ys_in_Z: "set ys \<subseteq> Z" and
     lasso_v_xs_ys: "lasso_from_node (induced_subgraph V\<^sub>\<alpha> \<sigma>) v xs ys"
     by blast+
   with Z_in_V have ys_in_V: "set ys \<subseteq> V" by simp
@@ -107,7 +47,7 @@ proof (intro ballI allI impI)
     y_in_ys: "y \<in> set ys" and
     ys_notempty: "ys \<noteq> []"
     by fastforce
-  with ys_in_Z have y_in_Z: "y \<in> ?Z" by blast
+  with ys_in_Z have y_in_Z: "y \<in> Z" by blast
 
   consider (A_in_ys) "set ys \<inter> A \<noteq> {}" | (A_notin_ys) "set ys \<inter> A = {}" by blast
   thus "winning_player ys" proof cases
@@ -126,10 +66,13 @@ proof (intro ballI allI impI)
     with winning_top_p show ?thesis by simp
   next
     case A_notin_ys
-    with tangles_T fin_T \<sigma>_attr_strat y_in_Z lasso_y_ys
-    show ?thesis by (auto simp: player_tangle_attractor_strat_def)
+    with player_tangle_attractor_strat[OF tangles_T fin_T attr] y_in_Z lasso_y_ys
+    show ?thesis by fastforce
   qed
 qed
+
+lemma "x \<notin> dom \<sigma> \<Longrightarrow> induced_subgraph V\<^sub>\<alpha> \<sigma> \<subseteq> induced_subgraph V\<^sub>\<alpha> (\<sigma>(x\<mapsto>y))"
+  unfolding induced_subgraph_def E_of_strat_def by force
 
 (** From anywhere in the tangle-attracted region Z to A, the opponent can reach a node of priority
     p (the top priority in the current region) *)
@@ -137,44 +80,63 @@ lemma van_dijk_3_player:
   assumes tangles_T: "\<forall>t\<in>T. player_tangle t"
   assumes fin_T: "finite T"
   assumes A_def: "A = {v. v\<in>V \<and> pr v = pr_set V}"
-  assumes \<sigma>_attr_strat: "player_tangle_attractor_strat T \<sigma> A"
-  shows "\<forall>v\<in>player_tangle_attractor T A. \<exists>v'. pr v' = pr_set V \<and> (\<exists>vs. path (induced_subgraph V\<^sub>\<alpha> \<sigma>) v  vs v')"
-proof (rule ballI)
-  fix v
-  assume "v \<in> player_tangle_attractor T A"
-  hence v_in_Attr: "v \<in> player_tangle_attractor T A" by simp
-  from tangles_T fin_T v_in_Attr show "\<exists>v'. pr v' = pr_set V \<and> (\<exists>vs. path (induced_subgraph V\<^sub>\<alpha> \<sigma>) v  vs v')"
-  proof (induction rule: player_tangle_attractor.induct)
-    (** x is itself a node with priority p, thus this case is true with an empty path. *)
-    case (base x)
-    show ?case
-      apply (rule exI[where x="x"]; rule conjI)
-        subgoal using A_def base by blast
-        subgoal by (rule exI[where x="[]"]) simp
+  assumes attr: "player_tangle_attractor T A Z \<sigma>"
+  shows "\<forall>v\<in>Z. \<exists>v'. pr v' = pr_set V \<and> (\<exists>vs. path (induced_subgraph V\<^sub>\<alpha> \<sigma>) v  vs v')"
+  using attr tangles_T fin_T
+proof (induction rule: player_tangle_attractor_induct')
+  case base thus ?case
+    apply (rule ballI)
+    subgoal for v
+      apply (rule exI[where x="v"]; rule conjI)
+      subgoal using A_def by simp
+      subgoal apply (rule exI[where x="[]"]) by simp
       done
-  next
-    (** It is not guaranteed that \<sigma>(x) = y, so there is no way to continue the proof here.
-        The induction does not know about \<sigma>, so we need a better induction that relates to \<sigma>. *)
-    case (own x y) thus ?case sorry, xxx sorry
-  next
-    case (opponent x)
-    then obtain y where
+    done
+next
+  case (own x S y \<sigma>)
+  show ?case proof (rule ballI)
+    fix v assume v_in_S': "v \<in> insert x S"
+    consider (x) "v=x" | (not_x) "v\<noteq>x" by blast
+    thus "\<exists>v'. pr v' = pr_set V \<and> (\<exists>vs. path (induced_subgraph V\<^sub>\<alpha> (\<sigma>(x\<mapsto>y))) v vs v')"
+    proof cases
+      case x
+      then show ?thesis sorry
+    next
+      case not_x
+      then show ?thesis sorry
+    qed
+  qed
+next
+  case (opponent x S \<sigma>)
+  show ?case proof (rule ballI)
+    fix v assume v_in_S': "v \<in> insert x S"
+    consider (x) "v=x" | (not_x) "v\<noteq>x" by blast
+    thus "\<exists>v'. pr v' = pr_set V \<and> (\<exists>vs. path (induced_subgraph V\<^sub>\<alpha> \<sigma>) v vs v')"
+    proof cases
+      case x with opponent obtain y where
       edge_in_E: "(x,y) \<in> E" and
       edge_in_subgraph: "(x,y) \<in> induced_subgraph V\<^sub>\<alpha> \<sigma>"
       using succ ind_subgraph_notin_dom
-      by fastforce
+      by blast
 
-    with opponent.IH obtain x' ys where
+    with opponent.IH opponent.hyps(2) obtain x' ys where
       pr_x': "pr x' = pr_set V" and
       path_y_ys_x': "path (induced_subgraph V\<^sub>\<alpha> \<sigma>) y ys x'"
       by blast
-
-    from path_y_ys_x' edge_in_subgraph have "path (induced_subgraph V\<^sub>\<alpha> \<sigma>) x (x#ys) x'" by auto
-    with pr_x' show ?case by blast
-  next
-    case (escape x t)
-    then show ?case sorry
+    from path_y_ys_x' edge_in_subgraph x have path_v_x':
+      "path (induced_subgraph V\<^sub>\<alpha> \<sigma>) v (x#ys) x'" by auto
+    show ?thesis
+      apply (rule exI[where x="x'"]; rule conjI)
+      subgoal using pr_x' .
+      subgoal apply (rule exI[where x="x#ys"]) using path_v_x' by blast
+      done
+    next
+      case not_x with v_in_S' opponent show ?thesis by blast
+    qed
   qed
+next
+  case (escape t S \<sigma>' \<sigma>)
+  show ?case sorry
 qed
 
 (** For each new tangle t, all successors of t are in higher \<alpha>-regions.
@@ -212,16 +174,15 @@ end (** End of context player_paritygame *)
 context paritygame begin
 
 (** The future proof still needs to show that this is limited to a region R, which is a subgame. *)
-lemma van_dijk_2':
+lemma van_dijk_2:
   assumes tangles_T: "\<forall>t\<in>T. tangle \<alpha> t"
   assumes fin_T: "finite T"
   assumes winning_top_p: "player_winningP \<alpha> (pr_set V)"
   assumes A_def: "A = {v. v\<in>V \<and> pr v = pr_set V}"
-  assumes \<sigma>_attr_strat: "tangle_attractor_strat \<alpha> T \<sigma> A"
-  shows "\<forall>v\<in>tangle_attractor \<alpha> T A.
-          \<forall>xs ys. lasso_from_node (induced_subgraph (V_player \<alpha>) \<sigma> \<inter> (tangle_attractor \<alpha> T A \<times> tangle_attractor \<alpha> T A)) v xs ys
+  assumes attr: "tangle_attractor \<alpha> T A Z \<sigma>"
+  shows "\<forall>v\<in>Z. \<forall>xs ys. lasso_from_node (induced_subgraph (V_player \<alpha>) \<sigma> \<inter> Z\<times>Z) v xs ys
             \<longrightarrow> player_wins_list \<alpha> ys"
-  using assms P0.van_dijk_2_player' P1.van_dijk_2_player'
+  using assms P0.van_dijk_2_player P1.van_dijk_2_player
   by (cases \<alpha>; simp)
 
 lemma van_dijk_7:
